\documentclass[a4paper]{article}
\input{../../../../../newpreamble.tex}
\title{Homework 8 Extra Credit}

\author{Lance Remigio}

\begin{document}
\maketitle

\begin{problem}
   Prove that  
   \[  \lim \inf {a}_{n} + \lim \inf {b}_{n} \leq \lim \inf({a}_{n} + {b}_{n}) \leq \lim \sup {a}_{n} + \lim \inf {b}_{n}  \]
   provided that all expressions are meaningful.
\end{problem}
\begin{proof}
Our goal is to show that 
\begin{enumerate}
    \item[(1)] \( \lim \inf {a}_{n} + \lim \inf {b}_{n} \leq \lim \inf({a}_{n} + {b}_{n})  \)
    \item[(2)]\( \inf({a}_{n} + {b}_{n}) \leq \lim \sup {a}_{n} + \lim \inf {b}_{n} \). 
\end{enumerate}
To show (1), we will assume that the left-hand side is NOT of the form \( \infty  + \infty   \). Hence, there exists \( n \geq {n}_{0}  \) and \( \ell \geq n  \) such that 
\begin{align*}
    {a}_{\ell} &\geq \inf \{ {a}_{k} : k \geq n  \},  \\
    {b}_{\ell} &\geq \inf \{ {b}_{k} : k \geq n \}. 
\end{align*}
Adding both inequalities above gives us 
\[  {a}_{\ell} + {b}_{\ell} \geq \inf \{ {a}_{k} : k \geq n  \}  + \inf \{ {b}_{k} : k \geq n  \}.  \]
Using the order limit theorem and algebraic limit theorem, we can write
\begin{align*}
    \lim_{ n \to \infty  }  \inf \{ {a}_{\ell } + {b}_{\ell} : \ell \geq n  \}   &\geq \lim_{ n \to \infty  }  [ \inf \{ {a}_{k } : k \geq n  \}  + \inf \{ {b}_{k } : k \geq n  \} ] \\
                                                                                 &= \lim_{ n \to \infty  }  \inf \{ {a}_{k } : k \geq n  \}  + \lim_{ n \to \infty  }  \inf \{ {b}_{k } : k \geq n  \}.
\end{align*}
Thus, we can conclude that 
\[  \lim \inf ({a}_{n} + {b}_{n}) \geq \lim \inf ({a}_{n}) + \lim \inf ({b}_{n}) \]
which establishes (1).

To show (2), we will consider the three cases; that is, 
\begin{itemize}
    \item \( \lim \inf ({a}_{n} + {b}_{n}) \neq -\infty \)
    \item \( \lim \sup {a}_{n} = \infty \)
    \item \( \lim \inf ({a}_{n} + {b}_{n}) \neq - \infty   \) and \( \lim \sup {a}_{n} \neq \infty \).
\end{itemize}

Suppose \( \lim \inf ({a}_{n} + {b}_{n}) \neq - \infty   \). If this is the case, the right-hand side of (2) will always hold. Next, suppose \( \lim \sup {a}_{n} = \infty \). Note that the right-hand side of (2) is NOT of the form \( \infty  + \infty   \). So, we can conclude that \( \lim \inf {b}_{n} \neq - \infty  \) and so 
\[ \lim \inf {b}_{n} + \lim \sup {a}_{n} = \infty. \]

Now, suppose that \( \lim \inf ({a}_{n} + {b}_{n}) \neq - \infty   \) and \( \lim \sup {a}_{n} \neq \infty \). Then using (1) and the algebraic limit theorem, we can write
\begin{align*}
    \lim \inf {b}_{n} &= \lim \inf [({b}_{n} + {a}_{n}) + (- {a}_{n})] \\
                      &\geq \lim \inf ({a}_{n} + {b}_{n}) + \lim \inf ({a}_{n}) \tag{ALT and (1)} \\
                      &= \lim \inf ({a}_{n} + {b}_{n}) - \lim \sup ({a}_{n})   \tag{Exercise 9}.
\end{align*}
Then we have 
\[  \lim \inf ({a}_{n} + {b}_{n}) \leq \lim \inf {b}_{n} + \lim \sup {a}_{n} \]
which establishes (2). Hence, we now conclude that 
   \[  \lim \inf {a}_{n} + \lim \inf {b}_{n} \leq \lim \inf({a}_{n} + {b}_{n}) \leq \lim \sup {a}_{n} + \lim \inf {b}_{n}  \]
\end{proof}

\begin{problem}
    Suppose \( X  \) is a nonempty complete metric space, and \( ({G}_{n}) \) is a sequence of dense open subsets of \( X  \). Prove Baire's Theorem, namely, \( \bigcap_{ n=1  }^{ \infty  }  {G}_{n}  \) is nonempty.
\end{problem}
\begin{proof}

\end{proof}

\begin{problem}
   Prove the following theorem: 
   \begin{center}
       Suppose \( ({s}_{n}) \) and \( ({b}_{n}) \) are two sequences of real numbers, \( ({b}_{n}) \) is a strictly increasing sequence that diverges to \( \infty   \), and \( \lim_{ n \to \infty  }  \frac{ {s}_{n+1} - {s}_{n}  }{ {b}_{n+1} - {b}_{n} } = L \in \R  \). Then \( \lim_{ n \to \infty  }  \frac{ {s}_{n} }{  {b}_{n} }  = L  \).
   \end{center}
\end{problem}
\begin{proof}
Suppose \( ({s}_{n}) \) and \( ({b}_{n}) \) are two sequences of real numbers and \( ({b}_{n}) \) is a strictly increasing sequence that diverges to \( \infty  \), and that 
\[  \lim_{ n \to \infty  }  \frac{ {s}_{n+1} - {s}_{n} }{  {b}_{n+1} - {b}_{n} }  =  L \in \R.  \]
Our goal is to show that \( \lim_{ n \to \infty  }  \frac{ {s}_{n} }{ {b}_{n} }  = L  \). In order to do this, we need to show that for any given \( \epsilon > 0  \), we have
\begin{align*}
    \lim \sup \frac{ {s}_{n} }{ {b}_{n} } &\leq L + \epsilon \tag{1}  \\
    \lim \inf \frac{ {s}_{n} }{ {b}_{n}  }  &\geq L + \epsilon \tag{2}
\end{align*}
To this end, let \( \epsilon > 0  \) be given. Since \( \lim_{ n \to \infty  }  \frac{ {s}_{n+1} - {s}_{n} }{  {b}_{n+1} - {b}_{n} }  = L  \), there exists an \( N \in \N  \) such that for any \( n > N \), we have 
\[  \Big|  \frac{ {s}_{n+1} - {s}_{n} }{  {b}_{n+1} - {b}_{n} } - L  \Big| < \epsilon \]
which can be written in the following way:
\[  (L-\epsilon) ({b}_{n+1} - {b}_{n}) < {s}_{n+1} - {s}_{n} < (L + \epsilon)({b}_{n+1} - {b}_{n}). \tag{*} \]
Now, fix an \( \hat{N} > N    \) denoted by \( \hat{N} = N + 2 \). Then observe that 
\[  {s}_{n} = [({s}_{n} - {s}_{n-1}) + ({s}_{n-1} - {s}_{n-2}) + \cdots + ({s}_{\hat{N}} - {s}_{\hat{N} - 1})] + {s}_{\hat{N} - 1}. \]
Applying (*) to the equation above gives us 
\begin{align*}
    {s}_{n} &< (L+\epsilon)[({b}_{n} - {b}_{n-1}) + ({b}_{n-1} - {b}_{n-2}) + \cdots + ({b}_{\hat{N}} - {b}_{\hat{N} -1})] + {s}_{\hat{N}-1} \\
            &= (L+\epsilon)[{b}_{n} - {b}_{\hat{N} - 1}] + {s}_{\hat{N} - 1}
\end{align*}
Multiplying by \( {b}_{n} \) on both sides, we get
\begin{align*} \frac{ {s}_{n} }{ {b}_{n} }  &< (L+\epsilon) \Big[ \frac{ {b}_{n} - {b}_{\hat{N} - 1} }{ {b}_{n} } \Big]  + \frac{ {s}_{\hat{N} - 1} }{ {b}_{n} } \\ 
    &= (L+\epsilon) +  \frac{ {s}_{\hat{N} -1} -  {b}_{\hat{N} -1} (L+\epsilon) }{ {b}_{n} } 
\end{align*}
Since we have \( ({b}_{n}) \) is a strictly increasing sequence that diverges to \( \infty   \), we must have \( \frac{ 1 }{ {b}_{n} }  \to 0  \). Since 
\[  \alpha = {s}_{\hat{N} - 1} - {b}_{\hat{N} - 1} (L+\epsilon)  \]
is a fixed quantity (because \( \hat{N} \) is fixed), we have that \( \frac{ \alpha }{ {b}_{n} } \to 0  \) by the algebraic limit theorem. By the order limit theorem, we can see that 
\begin{align*}
    \lim_{n \to \infty } \sup \frac{ {a}_{n} }{ {b}_{n} } &\leq  \lim_{ n \to \infty  }  \Big[ (L+\epsilon) + \frac{ \alpha  }{ {b}_{n} } \Big]  \\
                                                          &= (L+\epsilon) + \lim_{ n \to \infty  }  \frac{ \alpha }{ {b}_{n} } \tag{ALT}  \\
                                                          &= L+\epsilon + 0 \\ 
                                                          &= L + \epsilon.
\end{align*}
which establishes (1).

We can apply an analogous process to establish (2). By applying (*), we can see that 
\[ \frac{ {s}_{n} }{ {b}_{n} }  > (L - \epsilon) + \frac{ {s}_{\hat{N} - 1} - {b}_{\hat{N} - 1}(L-\epsilon) }{ {b}_{n} }.  \]
Now, set
\[  \beta = {s}_{\hat{N} - 1} - {b}_{\hat{N} - 1}(L - \epsilon). \]
By the order limit theorem, we see that 
\begin{align*}
    \lim_{ n \to \infty  }  \inf \frac{ {s}_{n} }{ {b}_{n} }  &\geq \lim_{ n \to \infty  }  \Big[ (L-\epsilon) + \frac{\beta}{ {b}_{n} } \Big]  \\
                                                              &= (L-\epsilon) + \lim_{ n \to \infty  }  \frac{ \beta }{ {b}_{n} } \tag{ALT}  \\
                                                              &= L - \epsilon + 0 \\
                                                              &= L - \epsilon
\end{align*} 
which establishes (2). Since \( \epsilon > 0  \) is arbitrary, (1) and (2) imply that 
\[  \lim \sup \frac{ {s}_{n} }{ {b}_{n} }  \leq L \ \ \text{and} \ \ \lim \inf \frac{  {s}_{n} }{ {b}_{n} } \geq L.   \]
Thus, we can see that
\[  \lim \sup \frac{ {s}_{n} }{ {b}_{n} }  = \lim \inf \frac{ {s}_{n} }{ {b}_{n} }  = L.   \]
This tells us that 
\[  \lim_{ n \to \infty  }  \frac{ {s}_{n} }{ {b}_{n} }  = L.  \]



\end{proof}



\end{document}
