\documentclass[a4paper]{report}
\usepackage{standalone}
\usepackage{import}

\input{../../../../../newpreamble.tex}


\begin{document}

\section{Lecture 4}

\subsection{Topics}

\begin{itemize}
    \item Continue discussion of convergence of sequences and series.
    \item Discuss exponential, sine, and cosine function.
\end{itemize}

\subsection{Class Exercises}

\begin{enumerate}
    \item[(i)] Show that \( \sum_{ n=0  }^{  \infty  } \frac{ z^{n} }{ n! }  \) converges for all \( z  \).
    \item[(ii)] Show that \( \sum_{ n= 0  }^{  \infty  } (-1)^{n} \frac{ z^{2n} }{ (2n)! }  \) converges for all \( z \).
    \item[(iii)] Show that \( \sum_{ n=0 }^{ \infty  } (-1)^{n} \frac{ z^{2n+1} }{ (2n+1)! }  \) converges for all \( z \).
\end{enumerate}

\begin{definition}[Exponential, Cosine, and Sine]
    We define 
    \begin{align*}
        \exp(z) &= \sum_{ n= 0  }^{  \infty  } \frac{ z^{n} }{ n! }  \\
        \cos(z) &= \sum_{ n=0 }^{ \infty  } \frac{ (-1)^{n} z^{2n} }{ (2n)! } \\
        \sin(z) &= \sum_{ n=0 }^{ \infty   } (-1)^{n} \frac{ z^{2n+1} }{ (2n+1)! }.
    \end{align*}
\end{definition}

Our main goal for this lecture is to show that \( \exp(z+w) = \exp(z) \exp(w) \).

\subsection{Cauchy Multiplication Theorem}

\begin{theorem}[Cauhcy Multiplication Theorem]
    Assume that \( \sum_{ n = 0  }^{  \infty  } {z}_{n} \) and \( \sum_{ n=0  }^{  \infty  } {w}_{n}  \) converges absolutely. Then 
    \[  \sum_{ n=0 }^{ \infty  } = \Big(  \sum_{  n = 0  }^{ \infty  } {z}_{n} \Big) \Big(  \sum_{ n= 0  }^{ \infty  } {w}_{n} \Big) \tag{1} \]
where the series in the left converges absolutely.
\end{theorem}
\begin{proof}
We will show that the sequence of partial sums of (1) satisfy the conditions of the monotone convergence theorem so that it converges. \textbf{Why is (1) monotone?} First, we show that (1) is bounded. Observe that
\begin{align*}
    \sum_{ n = 0    }^{ N  }  \Big|  \sum_{ i + j = n  }^{  } {z}_{i} {w}_{j} \Big|  &\leq \sum_{ n = 0  }^{ N  } \sum_{ i + j = n  }^{   } | {z}_{i} {w}_{j} |  \\
                                                                                     &= \sum_{ 0 \leq i + j \leq N   }^{  }| {z}_{i} {w}_{j} | \\ 
                                                                                     &\leq \sum_{ 0 \leq i, j \leq N  }^{  } | {z}_{i} {w}_{j} | \\
                                                                                     &= \sum_{i = 0  }^{ N  } | {z}_{i}  |  \sum_{ j=0  }^{ N  } | {w}_{j} |. 
\end{align*}
By our assumption, we can see that the sequence of partial sums of \( \sum_{ n= 0  }^{  \infty  }    \) and \( \sum_{ n = 0  }^{  \infty  } {w}_{n} \) are bounded, and thus the left side of the equation above is bounded. Thus, we see that 
\[  \sum_{ n = 0  }^{  N  } \Big|  \sum_{  i + j = n  }^{   } {z}_{i} {w}_{j} \Big|  \] 
converges by the monotone convergence theorem. Next, we will show that 
\[  {\alpha}_{n} = \Big|  \sum_{ n = 0  }^{ 2N  } \sum_{  i + j = n  } {z}_{i} {w}_{j} - \sum_{ i = 0  }^{ N  } {z}_{i} \sum_{ j = 0  } {w}_{j}  \Big| \to 0  \]
as \( N \to \infty  \). Let us define the following sets
\begin{align*}
    {T}_{N} &= \{ (i,j) \in \Z \times \Z : i \geq 0 , j \geq 0, 0 \leq i + j \leq N  \}  \\
    {t}_{n} &= \{ (i,j) \in \Z \times \Z : 0 \leq i \leq N , 0 \leq j \leq N  \}.
\end{align*}
Observe that \( {T}_{N} \subseteq  {t}_{n} \) and \( {t}_{N} \subseteq  {T}_{2N } \subseteq  {t}_{2N} \). Thus, 
\begin{align*}
    {\alpha}_{N} &= \Big|  \sum_{ (i,j) \in {T}_{2N} \setminus  {t}_{N} }^{  } {z}_{i} {w}_{j} \Big| \leq \sum_{ (i,j) \in {T}_{2N} \setminus {t}_{N} }^{  } | {z}_{i} {w}_{j} |  \\
                 &\leq \sum_{ (i,j) \in {t}_{2N} \setminus  {t}_{N} }^{  } | {z}_{i} {w}_{j} |  \\
                 &= \sum_{ i=0  }^{ 2N  } \sum_{ j = 0  }^{ 2N  } | {z}_{i} {w}_{j} |  - \sum_{ i = 0  }^{  N  } \sum_{ j = 0  }^{  N  } | {z}_{i} {w}_{j} |  \\
                 &= \sum_{ i = 0  }^{  2 N  } | {z}_{i} | \sum_{ j = 0  }^{  2N  } | {w}_{j} |  - \sum_{ i = 0  }^{  N  } | {z}_{i} |  \sum_{ j = 0  }^{  N  } | {w}_{j} | \to 0  \ \text{as} \ N \to \infty.
\end{align*}


\end{proof}

\begin{corollary}
   For any \( z,w \in \C  \), we have \( \exp(z) \cdot \exp(w) = \exp(z + w) \). 
\end{corollary}
\begin{proof}
Let
\[  {C}_{n} = \sum_{ k = 0  }^{ n  } \frac{ z^{k } }{  k!  }  \cdot \frac{ w^{n-k} }{ (n-k)! }. \]
Then multiplying by \( n!  \) on both sides of the equation above, we see that
\[  n! {C}_{n} = \sum_{ k = 0  }^{ n  } \begin{pmatrix} n \\ k  \end{pmatrix} z^{k } w^{n - k } = (z + w)^{n} \]
by the binomial formula where
\[  \begin{pmatrix} n \\ k  \end{pmatrix}  = \frac{ n!  }{ k! (n- k)! }. \]
Now, observe that
\[  \sum_{ n = 0  }^{  N  } {C}_{n} = \sum_{ n = 0  }^{  N  } \frac{ n! {C}_{n}  }{  n!  }  = \sum_{ n = 0  }^{  N  } \frac{ (z + w )^{n} }{ n!  }. \]
Let \( n \to \infty  \). Then we have
\[  \sum_{ n = 0  }^{  \infty  } {C}_{n} = \sum_{ n = 0  }^{  \infty  } \frac{ (z+w)^{n} }{ n!  }  = \exp(z+w). \]

\end{proof}


\section{Lecture 5}





\end{document}
