\section{Further Properties of Projections}

\begin{theorem}[Partial Order]\label{9.6-1}
    Let \( {P}_{1}  \) and \( {P}_{2} \) be projections defined on a Hilbert space \( H  \). Denote by \( {Y}_{1} = {P}_{1}(H) \) and \( {Y}_{2} = {P}_{2}(H) \), the subspaces onto which \( H  \) is projected by \( {P}_{1} \) and \( {P}_{2} \), and let \( N({P}_{1}) \) and \( N({P}_{2}) \) be the null spaces of these projections. Then the following conditions are equivalent.
    \begin{enumerate}
        \item[(1)] \( {P}_{2}{P}_{1} = {P}_{1} {P}_{2} = {P}_{1} \)
        \item[(2)] \( {Y}_{1} \subseteq {Y}_{2} \)
        \item[(3)] \( N({P}_{1}) \supseteq N({P}_{2}) \)
        \item[(4)] \( \|{P}_{1}x\| \leq \|{P}_{2}x \|  \) for all \( x \in H  \)
        \item[(5)] \( {P}_{1} \leq {P}_{2} \).
    \end{enumerate}
\end{theorem}
\begin{proof}
\( (1) \implies (4) \) From {\hyperref[9.5-2]{9.5-2}}, it follows that \( \|{P}_{1}\| \leq 1  \). Using (1), we can see that for all \( x \in H \)
\[  \|{P}_{1}x\| = \|{P}_{1} {P}_{2} x \| \leq \|{P}_{1}\| \|{P}_{2}x\| \leq \|{P}_{2}x\|.  \]
Hence, \( \|{P}_{1}x \| \leq \|{P}_{2}x \| \).

\( (4) \implies (5) \) Since \( \langle {P}_{1}x ,  x  \rangle = \|P_1 x\|^{2} \), it follows that for all \( x \in H  \)
\[  \langle {P}_{1}x  , x \rangle = \|{P}_{1}x \|^{2} \leq \|{P}_{2}x\|^{2} = \langle {P}_{2}x  ,  x  \rangle. \]
Thus, we have \( {P}_{1} \leq {P}_{2} \) by definition.

\( (5) \implies (3) \) Assume \( {P}_{1}\leq {P}_{2} \). Our goal is to show \( N({P}_{2}) \subseteq N({P}_{1})  \). Let \( x \in N({P}_{2}) \). Then \( {P}_{2}x = 0  \) by definition. Using the fact that \( \langle {P}_{1}x  ,  x  \rangle = \|{P}_{1}x\|^{2} \) and (5) from our theorem, it follows that 
\[  \|{P}_{1}x\|^{2} = \langle {P}_{1}x  ,  x  \rangle \leq \langle {P}_{2}x  ,  x  \rangle = 0.   \]
Thus, we can see that \( {P}_{1}x = 0  \) and so \( x \in N({P}_{1}) \) and \( N({P}_{2}) \subseteq N({P}_{1})  \).

  \( (3) \implies (2) \) By {\hyperref[3.3-5]{3.3-5}}, since \( N({P}_{j})   \) is the orthogonal complement of \( {Y}_{j} \) in \( H  \), it immediately follows that \( {Y}_{1} \subseteq {Y}_{2} \). 

  \( (2) \implies (1) \) Assume \( {Y}_{1} \subseteq {Y}_{2} \). For every \( x \in H  \), we have \( {P}_{1}x \in {Y}_{1} \). Thus, \( {P}_{1}x \in {Y}_{2} \) by assumption and so we have 
  \[  {P}_{2}({P}_{1}x) = {P}_{1}x.   \]
  Thus, \( {P}_{2}{P}_{1} = {P}_{1} \). Note that since \( {P}_{1} \) is a projection, \( {P}_{1} \) must also be self-adjoint by {\hyperref[9.5-1]{9.5-1}}. Using {\hyperref[3.10-4]{3.10-4}}, we see immediately that   
  \[  {P}_{1} = {P}_{2}{P}_{1} = {P}_{1} {P}_{2}. \]
\end{proof}


\begin{theorem}[Difference of Projections]\label{9.6-2}
    Let \( {P}_{1}  \) and \( {P}_{2} \) be projections on a Hilbert space \( H  \). Then:
    \begin{enumerate}
        \item[(a)] The difference \( P = {P}_{2} - {P}_{1} \) is a projection on \( H  \) if and only if \( {Y}_{1} \subseteq  {Y}_{2} \), where \( {Y}_{j} = {P}_{j}(H) \).
        \item[(b)] If \( P = {P}_{2} - {P}_{1} \), then \( P  \) projects \( H  \) onto \( Y  \), where \( Y  \) is the orthogonal complement of \( {Y}_{1} \) in \( {Y}_{2} \).
    \end{enumerate}
\end{theorem}
\begin{proof}
\begin{enumerate}
    \item[(a)] \( (\Longrightarrow) \) Suppose \( P = {P}_{2} - {P}_{1} \) is a projection on \( H  \). Our goal is to show that \( {Y}_{1} \subseteq {Y}_{2} \). Our strategy is to prove that 
        \[  {P}_{2}{P}_{1} = {P}_{1} {P}_{2} = {P}_{1} \]
        so that we may apply {\hyperref[9.6-1]{9.6-1}} to obtain our result. By assumption, we see that \( P^{2} = P  \) by {\hyperref[9.5-1]{9.5-1}} and so we obtain
        \[  {P}_{2} - {P}_{1} = ({P}_{2} - {P}_{1})^{2} = {P}_{2}^{2} - {P}_{2} {P}_{1} - {P}_{1} {P}_{2} + {P}_{1}^{2}.\]
        On the right-hand side, since \( {P}_{1} \) and \( {P}_{2} \) are also projections, we have \( {P}_{2}^{2} = {P}_{2} \) and \( {P}_{1}^{2} = {P}_{1} \) by {\hyperref[9.5-1]{9.5-1}}. And so the above equation enables us to write
        \[  {P}_{1}{P}_{2} = {P}_{2}{P}_{1} = 2 {P}_{1}. \tag{I} \]
        Multiplying \( {P}_{2} \) on the left-hand side of (I) gives us
        \[  {P}_{2}{P}_{1} {P}_{2} + {P}_{2}{P}_{1} = 2 {P}_{2} {P}_{1}. \]
        Then we have
        \[  {P}_{2} {P}_{1} {P}_{2} = {P}_{2} {P}_{1}. \tag{1} \]
        Multiplying \( {P}_{2}  \) on the right-hand side of (I) gives us
        \[ {P}_{1}{P}_{2} + {P}_{2} {P}_{1} {P}_{2} = 2 {P}_{1} {P}_{2}.  \]
        Then we have 
        \[  {P}_{2} {P}_{1} {P}_{2} = {P}_{1} {P}_{2}. \tag{2} \]
        From (1) and (2), it follows that 
        \[  {P}_{2} {P}_{1} = {P}_{1} {P}_{2} = {P}_{1} \]
        which is our desired result.
       
        \( (\Longleftarrow) \) Our goal is to show that \( P  \) is idempotent and \( P  \) is self-adjoint by {\hyperref[9.5-1]{9.5-1}}. If \( {Y}_{1} \subseteq {Y}_{2} \), we see from {\hyperref[9.6-1]{9.6-1}} that \( {P}_{2}{P}_{1} = {P}_{1} {P}_{2} = {P}_{1} \) which further implies that 
        \[  {P}_{1}{P}_{2} + {P}_{2} {P}_{1} = 2 {P}_{1} \]
        and consequently shows that \( P \) is idempotent. Indeed, we see that  
        \begin{align*}
            P^{2} = ({P}_{2} - {P}_{1})^{2} 
                  &= {P}_{2}^{2} - ({P}_{2} {P}_{1} + {P}_{1} {P}_{2}) + {P}_{1}^{2} \\
                  &= {P}_{2} - ({P}_{2} {P}_{1} + {P}_{1} {P}_{2}) + {P}_{1} \\
                  &= {P}_{2} - {P}_{1} \\
                  &= P.
        \end{align*}
        Hence, \( P^{2} = P  \).
        Since \( {P}_{1} \) and \( {P}_{2} \) are self-adjoint, it follows that \( P = {P}_{2} - {P}_{1} \) is also self-adjoint, and so \( P  \) is a projection.
    \item[(b)] Our goal is to show that \( Y  = V =  {Y}_{2} \cap {Y}_{1}^{\perp}  \). Note that \( Y = P(H) \) consists of all vectors of the form 
        \[  y = Px = {P}_{2}x - {P}_{1}x \]
        for all \( x \in H \). Suppose \( P = {P}_{2} - {P}_{1} \) is a projection. Then from part (a), it follows that \( {Y}_{1} \subseteq {Y}_{2} \) and so we have \( {P}_{2} {P}_{1} = {P}_{1} \). Thus, we obtain from the above equation that 
        \[  {P}_{2} y = {P}_{2}^{2} x - {P}_{2} {P}_{1} x = {P}_{2} x - {P}_{1} x = y.  \]
        This tells us that \( y \in {Y}_{2} \). Similarly, we have   
        \[  {P}_{1}y = {P}_{1}{P}_{2}x - {P}_{1}^{2}x = {P}_{1}x - {P}_{1}x = 0.  \]
        This tells us that \( y \in N({P}_{1}) = {Y}_{1}^{\perp} \) by \( {\hyperref[3.3-5]{3.3-5}}  \). Together, \( y \in V  \) where \( V = {Y}_{2} \cap {Y}_{1}^{\perp} \). Since \( y \in Y  \) was arbitrary, we have \( Y \subseteq V  \) 

        Now, we will show that \( V \subseteq Y  \). Observe that the projection of \( H  \) onto \( {Y}_{1}^{\perp}  \) is \( I - {P}_{1} \), and so for every \( v \in V  \), we can see that 
        \[  v = (I - {P}_{1}){y}_{2}. \]
        Using \( {P}_{2} {P}_{1} = {P}_{1} \), we obtain from the above equation that, since \( {P}_{2} {y}_{2} = {y}_{2} \), we have 
        \begin{align*}
            Pv &= ({P}_{2} - {P}_{1}) (I - {P}_{1}){y}_{2}  \\
               &= ({P}_{2} - {P}_{2} {P}_{1} - {P}_{1} + {P}_{1}^{2}) {y}_{2} \\
               &= ({P}_{2} - {P}_{2}{P}_{1}){y}_{2} \\
               &= {P}_{2}{y}_{2} - ({P}_{2} {P}_{1}){y}_{2} \\
               &= (I - {P}_{1}){y}_{2} \\
               &= v.
        \end{align*}
        Hence, we have \( v \in Y  \) and so \( V \subseteq Y  \) since \( v  \) is arbitrary. Together, we identify \( Y = P(H) \) with \( V = {Y}_{2} \cap {Y}_{1}^{\perp} \).
\end{enumerate}
\end{proof}


\begin{theorem}[Monotone Increasing Sequence]
    Let \( ({P}_{n}) \) be a monotone increasing sequence of projections \( {P}_{n} \) defined on a Hilbert space \( H  \). Then:
    \begin{enumerate}
        \item[(a)] \( ({P}_{n}) \) is strongly operator convergent, say, \( {P}_{n}x \to Px   \) for every \( x \in H  \), and the limit operator \( P  \) is a projection defined on \( H  \).
        \item[(b)] \( P \) projects \(H  \) onto 
            \[  P(H) = \overline{\bigcup_{ n=1  }^{ \infty  }  {P}_{n}(H) }. \]
        \item[(c)] \( P  \) has the null space 
            \[  N(P) = \bigcap_{ n=1  }^{ \infty  }  N({P}_{n}). \]
    \end{enumerate}
\end{theorem}
    \begin{proof}
    \begin{enumerate}
        \item[(a)] Let \( m < n  \). By assumption, we can see that \( {P}_{m} \leq {P}_{n}  \) so that we have \( {P}_{m}(H) \subseteq  {P}_{n}(H) \) by {\hyperref[9.6-1]{9.6-1}} and \( {P}_{n} - {P}_{m}  \) is a projection by {\hyperref[9.6-2]{9.6-2}}. Hence, for every fixed \( x \in H  \), we get via {\hyperref[9.5-2]{9.5-2}} that 
            \begin{align*}
                \|{P}_{n}x -  {P}_{m}x\|^{2} &= \|({P}_{n} - {P}_{m})x\|^{2} \\
                                             &= \langle ({P}_{n} - {P}_{m})x  ,  x \rangle \\
                                             &= \langle {P}_{n} x  ,  x  \rangle - \langle {P}_{m}x  , x  \rangle \\
                                             &= \|{P}_{n}x\|^{2} - \|{P}_{m}x\|^{2}.
            \end{align*}
            Using {\hyperref[9.5-2]{9.5-2}}, we get \( \|{P}_{n}\| \leq 1  \) and so \( \|{P}_{n}x \| \leq \|x \|  \) for every \( n \in \N \). This tells us that \( \|{P}_{n}x\| \) is a bounded sequence of numbers. Also, \( (\|{P}_{n}x\|) \) is a monotone sequence by {\hyperref[9.6-1]{9.6-1}}. By the Monotone Convergence Theorem, it follows that \( \|{P}_{n}x\| \) is a convergent sequence and hence \( (\|{P}_{n}x\|) \) is a Cauchy sequence. As a consequence, \( ({P}_{n})  \) is also a Cauchy sequence in \( H  \) and so using the completeness of \( H  \) allows us to now say that \( {P}_{n}x \to Px   \) for some \( Px  \) in \( H  \). It is immediate that \( P  \) must be a projection on \( H  \) since is linear, self-adjoint and idempotent by {\hyperref[9.5-3]{9.5-3}} 
        \item[(b)] Our goal is to show that 
            \[  P(H) = \overline{\bigcup_{ n=1  }^{ \infty  }  {P}_{n}(H)}. \]
            Let \( m < n  \). Then \( {P}_{m} \leq {P}_{n} \), that is, \( {P}_{n} - {P}_{m} \geq 0  \) and so \( \langle ({P}_{n} - {P}_{m})x  , x  \rangle \geq 0  \) by definition. Letting \( n \to \infty   \), we obtain \( \langle (P - {P}_{m})x  ,  x  \rangle \geq 0  \) using the continuity of the inner product {\hyperref[3.2-2]{3.2-2}}; that is, we have \( {P}_{m} \leq P  \) and so {\hyperref[9.6-1]{9.6-1}} gives us \( {P}_{m}(H) \subseteq P(H)  \) for every \( m  \). Thus, we have 
            \[  \bigcup {P}_{m}(H) \subseteq P(H). \]
            Furthermore, for every \( m  \) and for every \( x \in H  \), we have 
            \[  {P}_{m}x \in {P}_{m}(H) \subseteq \bigcup {P}_{m}(H). \]
            Since \( {P}_{m}x \to Px  \), we see from {\hyperref[1.4-6]{1.4-6(a)}} that \( Px \in \overline{\bigcup {P}_{m}(H) } \). Hence, we have 
            \[  \bigcup {P}_{m}(H) \subseteq P(H) \subseteq \overline{ \bigcup {P}_{m}(H) }. \]
            From {\hyperref[3.3-5]{3.3-5}} , it follows that \( P(h) = N(I - P) \) so that \( P(H) \) is closed by \( {\hyperref[2.7-10]{2.7-10(b)}}  \). This implies that from the above containments that (since \( P(H) \) is closed)
            \[ \overline{\bigcup {P}_{m}(H) } \subseteq P(H)  \]
            Together, we see that 
            \[ P(H) = \overline{\bigcup {P}_{m}(H) }.\]
        \item[(c)] We determine \( N(P)  \). Using \( {\hyperref[3.3-5]{3.3-5}}  \), we see that 
            \[  N(P) = P(H)^{\perp} \subseteq {P}_{n}(H)^{\perp} \] for every \( n \in \N \) due to part (b). Hence, we have 
            \[  N(P) \subseteq \bigcap {P}_{n}(H)^{\perp} = \bigcap N({P}_{n}).  \]
            On the other hand, if \( x \in \bigcap N({P}_{n}) \), then \( x \in N({P}_{n}) \) for every \( n  \) so that \( {P}_{n}x = 0  \) and so \( {P}_{n}x \to Px  \) implies that \( Px = 0  \); that is, \( x \in   N(P) \). Thus, we see that 
            \[ \bigcap N({P}_{n}) \subseteq N(P). \]
            Together, we obtain our result that 
            \[ N(P) = \bigcap N({P}_{n}). \]
            

    \end{enumerate}
    \end{proof}
