\section{The Algebraic and Order Limit Theorems}

\subsubsection{Exercise 2.3.1} Let \( x_n \geq 0\) for all \( n \in \N \).

\begin{enumerate}
    \item[(a)] If \( (x_n ) \to 0 \), show that \( \sqrt{x_n} \to 0\).
        \begin{proof}
            Suppose \( x_n \geq 0 \) and \( x_n \to 0\). In order to show that \( \sqrt{x_n} \to 0\), it suffices to show that for every \( \epsilon> 0\), there exists an \( N \in \N \) such that for every \( n \geq N \) we have 
            \[ | \sqrt{x_n} - 0  | < \epsilon.\]
            Choose \( N \in \N\). Suppose \( x_n = 0 \) for all \( n \in \N \), then \( ( \sqrt{x_n}) = 0 \) for all \( n \geq N \) which means that \( ( \sqrt{x_n}) \to 0\). Suppose \( x_n > 0 \) for all \( n \in \N\), then observe that since \( (x_n) \to 0\)  and \( (x_n)\) bounded, we have 
            \begin{align*}
             | \sqrt{x_n} - 0 | &= | \sqrt{x_n} | \\
                            &= \Big| \frac{x_n}{ \sqrt{x_n}} \Big| \\
                            &=  \Big| \frac{x_n - 0}{ \sqrt{x_n}} \Big| \\ 
                            &=  \frac{|x_n - 0|}{ \sqrt{x_n}}  \\
                            &< \sqrt{M} \frac{ \epsilon }{ \sqrt{M} }  \\ 
                            &= \epsilon 
            \end{align*}
            Hence, it follows that \( ( \sqrt{x_n}) \to 0\).
        \end{proof}
    \item[(b)] If \( (x_n) \to x\), show that \( (\sqrt{x_n}) \to \sqrt{x}\).
        \begin{proof}
            Suppose that \( x_n \geq 0\) for all \( n \in \N \). Suppose \( (x_n) \to x \). We want to show that \( ( \sqrt{x_n}) \to x\). Suppose \( x_n = 0 \) and suppose \( N \in \N \) such that for every \( n \geq N \), then we have the first case above where \( x=0\) and \( ( \sqrt{x_n}) \to 0\). Now suppose \( x_n > 0 \) and choose \( N \in \N \) such that for every \( n \geq N \), then observe that since \( (x_n ) \to x \) and \( (x_n)\) is bounded by an integer \( M > 0 \), we have that 

        \begin{align*}
        |  \sqrt{x_n } - \sqrt{x}  | &= \Big| \frac{ x_n - x}{ \sqrt{x_n} + \sqrt{x}} \Big| \\
                          &= \frac{ | x_n - x |}{ |\sqrt{x_n} + \sqrt{x} | } \\
                          &< ( \sqrt{M} + \sqrt{x}) \frac{ \epsilon }{ (\sqrt{M} + \sqrt{x})} \\ 
                          &= \epsilon. 
        \end{align*}
        Hence, it follows that \( ( \sqrt{x_n}) \to \sqrt{x}\).
        \end{proof}
\end{enumerate}

\subsubsection{Exercise 2.3.2}
Using only Definition 2.2.3, prove that if \( (x_n) \to 2\), then 
\begin{enumerate}
    \item[(a)] \(  \Big(\frac{2x_n - 1}{ 3} \Big) \to 1\);
        \begin{proof}
            Suppose \( (x_n) \to 2\). Our goal is to show that property above. It suffices to show that for every \( \epsilon  > 0\), there exists \( N \in \N  \) such that for every  \( n \geq N  \), we have 
            \[ \Big| \frac{2x_n - 1}{3} - 1 \Big| < \epsilon. \]
        Choose \( N \in \N \) and suppose \( n \geq N \)
        \begin{align*}
        \Big| \frac{2x_n  - 1}{3} - 1 \Big| &= \Big| \frac{2x_n - 4}{3}  \Big| \\
                                    &= \Big| \frac{2}{3} (x_n - 2)\Big| \\
                                    &= \Big| \frac{2}{3} \Big| | x_n - 2 | \\ 
                                    &< \frac{2}{3} \cdot \frac{3 \epsilon }{2} \\
                                    &= \epsilon.
        \end{align*}
        Hence, it follows that 
        \[ \Big(  \frac{2x_n  - 1}{3}\Big) \to 1.\]
        \end{proof}
    \item[(b)] \( \Big(   \frac{1}{x_n}\Big) \to \frac{1}{2}\).
        \begin{proof}
        We want to show that for every \( \epsilon  > 0 \), there exists \( N \in \N \) such that for every \( n \geq N \), we have 
        \[ \Big| \frac{1}{x_n} - \frac{1}{2}\Big| < \epsilon.\]
        Choose \( N \in \N \) and assume \( n \geq N \). Since \( (x_n) \to 2\), we can write 
        \begin{align*}
        \Big| \frac{1}{x_n} - \frac{1}{2} \Big| &= \Big| \frac{2 - x_n}{2x_n} \Big| \\
                                                &= \frac{ | x_n - 2 |}{ 2|x_n |}. \tag{1} \\
        \end{align*}
        Since \( (x_n) \to 2\), we can set \( \epsilon  = 1\) so that we can lower bound the denominator of (1) using 
        \[ 2 - \epsilon < | x_n | \implies 1 < | x_n |. \]
        Then we can set \( N = \max \{ 1, \epsilon / 2 \}\) so that 
        \[ \frac{ | x_n - 2  |}{ 2| x_n |} < \frac{2 \epsilon }{2} = \epsilon \]
        which satisifes our desired property.
        \end{proof}

\end{enumerate}

\subsubsection{Exercise 2.3.3}
Let \( (x_n)  \) and \( (y_n) \) be given, and define \( (z_n) \) to be the "shuffled" sequence \( (x_1, y_1, x_2, y_2, x_3, y_3, \dots x_n, y_n, \dots ). \) Prove that \( (z_n) \) is convergent if and only if \( (x_n) \) and \( (y_n) \) are both convergent with \( \lim x_n = \lim y_n \).
\begin{theorem}{Squeeze Theorem}{}
        If \( x_n \leq y_n \leq z_n\) for all \( n \in \N \), and if \( \lim x_n = \lim z_n = \ell\), then \( \lim y_n = \ell\).
    \end{theorem}
\begin{proof}
    Suppose \( x_n \leq y_n \leq z_n\) for all \( n \in \N \) and suppose \( \lim x_n = \lim z_n = \ell\). We want to show that \( \lim y_n = \ell\). By the Order Limit Theorem, we have \( x_n \leq y_n \leq z_n \) for all \( n \in \N \) implies that \( \ell \leq y_n \leq \ell\) for all \( n \in \N \). But this means that \( y_n = \ell\) for all \( n \in \N \). Hence, for every \( \epsilon  > 0\), there exists an \( N \in \N\) such that for every \( n \geq N\) 
    \[ | y_n - \ell | = | \ell - \ell | = 0 < \epsilon.\]
    Hence, it follows that \( \lim y_n = \ell\).
\end{proof}

\subsubsection{Exercise 2.3.4}
Let \( (a_n) \to 0\), and use the Algebraic Limit Theorem to compute each of the following limits (assuming the fractions are always defined).
\begin{enumerate}
    \item[(a)] \( \lim \Big( \frac{1 + 2a_n}{ 1 + 3a_n - 4a_n^2}   \Big) \)
        \begin{proof}[Solution]
        Let \( (a_n) \to 0\). Then
        \begin{align*}
            \lim \Big( \frac{ 1 + 2a_n}{ 1 + 3a_n - 4a_n^2 } \Big) &= \frac{ \lim (1 + 2a_n)}{ \lim (1 + 3a_n - 4a_n^2)} \\
                                 &= \frac{ \lim 1 + \lim (2a_n)}{ \lim 1 + \lim (3a_n) - \lim (4a_n^2)} \\
                                 &= \frac{ 1 + 2 \cdot 0}{ 1 + 3 \cdot 0 + 4 \cdot 0^2} \\
                                 &= 1.
        \end{align*}
        \end{proof}
    \item[(b)] \( \lim \Big( \frac{ (a_n + 2)^2 - 4}{a_n} \Big)\)
        \begin{proof}[Solution]
        Let \( (a_n) \to 0\). Then 
        \begin{align*}
          \lim  \Big( \frac{ (a_n + 2)^2 - 4}{ a_n} \Big)&= \lim \Big( \frac{a_n^2 + 4a_n}{a_n} \Big) \\
                                                 &= \lim \Big( a_n + 4 \Big) \\  
                                                 &= \lim a_n + \lim 4 \\ 
                                                 &= 0 + 4 \\ 
                                                 &= 4.
        \end{align*}
        \end{proof}
    \item[(c)] \( \lim \Big( \frac{ \frac{2}{a_n} + 3}{ \frac{1}{a_n} + 5} \Big)\).
        \begin{proof}[Solution]
        Let \( (a_n) \to 0\). Then 
        \begin{align*}
        \lim \Big( \frac{ \frac{2}{a_n} + 3}{ \frac{1}{a_n} + 5} \Big) &= \lim \Big( \frac{2 + 3a_n}{1 + 5a_n} \Big)  \\
                                                               &= \frac{ \lim 2 + \lim (3a_n)}{ \lim 1 + \lim (5a_n)} \\ 
                                                               &= \frac{2 + 3 \cdot 0}{ 1 + 5 \cdot 0}\\
                                                               &=2. 
        \end{align*}
        \end{proof}
\end{enumerate}

\subsubsection{Exercise 2.3.5}
Let \( (x_n)\) and \( (y_n)\) be given, and define \( (z_n)\) to be the "shuffled" sequence \[ (x_1, y_1, x_2, y_2 ,...,x_n, y_n).\] 
For the forwards direction, assume \( (z_n) \) is a convergent sequence. We want to show that \( \lim x_n = \lim y_n \). It suffices to show that given any \( \epsilon > 0\), there exists an \( N \in \N \) such that for any \( n \geq N \), we have 
\[ | x_n - y_n | < \epsilon.\]
Suppose \( (x_n) \to x\) and \( (y_n) \to y\), then we can write 
\begin{align*}
   | x_n - y_n  | &= | x_n - z_n + z_n - y_n |  \\
                  &< | x_n - z_n | + | z_n - y_n | \\  
                  &= | x_n - z + z - z_n | + | z_n - z + z - y_n | \\
                  &< | x_n - x | + | x - z_n | + | z_n - y | + | y - y_n |. \tag{1} 
\end{align*}
By definition, \( (z_n)\) is a shuffled sequence and convergent. Hence, \( z_n \to x \) and \( z_n \to y\). But by the uniqueness of limits, \( x = y\) so we have that 
\[ | x_n - y_n | < \frac{ \epsilon }{4} + \frac{ \epsilon }{4} +  \frac{ \epsilon }{4} + \frac{ \epsilon }{4} = \epsilon.\]
which means \( \lim (x_n - y_n) = \lim x_n - \lim y_n = 0\). 

Now for the backwards direction, assume \( \lim x_n = \lim y_n\). We want to show \( (z_n)\) converges i.e for every \( \epsilon> 0\), there exists \( N \in \N \) such that for every \( n \geq N \), we have 
\[ | z_n - z | < \epsilon.\]

\subsubsection{Exercise 2.3.6} 
Consider the sequence given by \( b_n = n - \sqrt{n^2 + 2n}\). Taking \( (1 / n ) \to 0\) as given, and using both the Algebraic Limit Theorem and the result in Exercise 2.3.1, show \( \lim b_n \) exists and find the value of the limit.

\begin{proof}
Consider the sequence given by \( b_n = n - \sqrt{n^2 + 2n}\). Assume \( (1 / n ) \to 0\) and \( \sqrt{x_n} \to \sqrt{x} \). Then taking the limit of \( b_n\), we have 
\begin{align*}
    \lim b_n &= \lim (n - \sqrt{n^2 + 2n}) \\
             &= \lim   \frac{-2n}{n + \sqrt{n^2 + 2n}} \\  
             &= \lim \frac{ -2}{ 1 + \sqrt{1 + 2 / n}} \\
             &= \frac{ \lim (-2) }{ \lim (1 + \sqrt{1 + 2 / n})} \\
             &= \frac{\lim(-2)}{\lim (1) + \lim (\sqrt{1 + 2 / n})} \\
             &= \frac{-2}{1 + 1 + 0} \tag{\((1/n) \to 0\), \( (\sqrt{x_n}) \to \sqrt{x} \) } \\
             &= -1.
\end{align*}
Hence, we have \( \lim b_n = -1 \). Now we can show that \( b_n\) does reach this limit. 

Let \( \epsilon > 0\). Then choose 
\[ N = \frac{2}{ \sqrt{ \frac{1 + \epsilon }{1 - \epsilon }} - 1}.\]
Then assumme \( n \geq N \). Our goal is to show that 
\[ | b_n + 1 | < \epsilon.\]
Then 
\begin{align*}
    &n >  \frac{2}{ \sqrt{ \frac{1 + \epsilon }{1 - \epsilon }} - 1} \\
    \implies &\sqrt{ \frac{1 + \epsilon }{1 - \epsilon }} -1  > \frac{2}{n}  \\  
\end{align*} Then we have 
\begin{align*}
  \sqrt{1+2/n}  &< \frac{1 + \epsilon }{1 - \epsilon } \\
  (1 - \epsilon )\sqrt{1 - 2/n} &< 1 + \epsilon \\   
  (1 - \epsilon )\sqrt{1 - 2/n} - 1 &< \epsilon .
\end{align*}
Then we get 
\begin{align*}
    - 1 + \sqrt{1 + 2 / n} < \epsilon ( 1 + \sqrt{ 1 + 2 / n})     \\
\end{align*}
and then 
\begin{align*}
    \frac{ - 1 + \sqrt{1 + 2/n}}{ 1 + \sqrt{ 1 + 2/n}} &< \epsilon \\ 
    \frac{ -2n}{ n + \sqrt{ n^2 + 2n}} + \frac{n + \sqrt{n^2 + 2n}}{ n + \sqrt{ n^2 + 2n}} &< \epsilon \\ 
    n - \sqrt{n^2 + 2n} + 1 &< \epsilon.
\end{align*}
Hence, it follows that \( | b_n + 1  | < \epsilon\).

\end{proof}

\subsubsection{Exercise 2.3.8}
Let \( (x_n) \to x \) and let \( p(x)\) be a polynomial.
\begin{enumerate}
    \item[(a)] Show \( p(x_n) \to p(x)\).
        \begin{proof}
            Let \( (x_n) \to x \) and let \( p(x)\) be a polynomial. Let 
            \[ p(x) = \sum_{i=0}^{m} a_i x^i\]
            and 
            \[ p(x_n) = \sum_{i=0}^{m} a_i x_n^{i}. \]
            Our goal is to show that for every \( \epsilon > 0\), there exists \( N \in \N \) such that for every \( n \geq N \)            we have 
            \[ | p(x_n) - p(x)| < \epsilon.\]
           Then by part (i) of the Algebraic Limit Theorem, we have
           \begin{align*}
            | p(x_n) - p(x) |  &= \Big| \sum_{i=0}^{m} a_i x_n^{i} - \sum_{i=0}^{ m} a_i x^{i}  \Big| \\
                               &= \Big| \sum_{i=0}^{m} a_i (x^i_n - x^i)  \Big| \\
                               &<  \sum_{ i = 0}^{ m} | a_ix^i_n - a_ix^i | \tag{T.I}\\     
                               &<  \sum_{i=0}^{m} \frac{ \epsilon }{ m}  \tag{\(x_n \to x\)} \\
                               &= \frac{ \epsilon }{m }  \cdot m \\ 
                               &= \epsilon. 
           \end{align*}
           Hence, we have \( p(x_n) \to p(x)\).

        \end{proof}
    \item[(b)] Find an example of a function \( f(x)\) and a convergent sequence \( (x_n) \to x\) where the sequence \( f(x_n)\) converges, but not to \( f(x)\).
        
\end{enumerate}

\subsubsection{Exercise 2.3.9}
\begin{enumerate}
    \item[(a)] Let \( (a_n)\) be a bounded (not necessarily convergent) sequence, and assume \( \lim b_n  = 0\). Show that \( \lim (a_n b_n) = 0\). Why are we not allowed to use the Algebraic Limit Theorem to prove this? 
        \begin{proof}
        Let \( (a_n)\) be a bounded but not necessarily convergent sequence, and assume \( \lim b_n = 0 \). We want to show that \( \lim (a_n b_n ) = 0\). It suffices to show that for every \( \epsilon  > 0\), there exists \( N \in \N\) such that for every \( n \geq N \), we have 
        \[ | a_nb_n - 0 | < \epsilon. \tag{1}\]
        Since \( (a_n)\) bounded, there exists an \( M > 0\) such that \( | a_n  | < M \). Starting with the left side of (1), choose \( N \in \N \) such that for every \( n \geq N \) 
        \begin{align*}
            | a_n b_n - 0 |&= | a_n | | b_n |\\
                           &< M \cdot \frac{ \epsilon }{M} \tag{\(b_n \to 0\)} \\ 
                           &= \epsilon. 
        \end{align*}
        Hence, it follows that \( \lim (a_n b_n) \to 0\). We cannot use the Algebraic Limit Theorem here because \( (a_n)\) does not necessarily have a defined limit even though it is bounded.
        \end{proof}
    \item[(b)] Can we conclude anything about the convergence of \( (a_nb_n)\) if we assume that \( (b_n)\) converges to some nonzero limit \( b \)?
        \begin{proof}[Solution]
        It would simply not converge.
        \end{proof}
    \item[(c)] Use (a) to prove Theorem 2.3.3, part (iii), for the case when \( a = 0\). 
        \begin{proof}
            Suppose \( a_n \to a\) where \( a = 0\) and \( b_n \to b\). Our goal is to show that \( \lim(a_n b_n) = 0\). Let \( \epsilon > 0 \), then choose \( N \in \N \) such that for every \( n \geq N \),  
        \begin{align*}
         | a_nb_n - 0| &< | a_n | | b_n |   \\
                       &< \frac{ \epsilon }{ M } \cdot M  \tag{\( a_n \to 0, b_n \to b\)} \\ 
                       &< \epsilon   
        \end{align*}
        Hence, it follows that \( \lim (a_nb_n) = 0\).
        \end{proof}
\end{enumerate}

\subsubsection{Exercise 2.3.10} Consider the following list of conjectures. Provide a short proof that are true and a counterexample for any that are false.
\begin{enumerate}
    \item[(a)] If \( \lim (a_n - b_n) = 0 \), then \( \lim a_n = \lim b_n\). 
        \begin{proof}[Counterexample]
        Suppose \( a_n = \frac{n}{2n+1}\) and \( b_n = \frac{n}{2n+5}\). We have \( \lim a_n = \lim b_n \) but \( \lim (a_n - b_n ) \neq 0\).
        \end{proof}
    \item[(b)] If \( (b_n) \to b\), then \( | b_n | \to | b |\).
        \begin{proof}
        Let \( \epsilon > 0\). Consider \( | |b_n| - |b|| \). Assume \( n \geq N \) then 
        \begin{align*}
           | |b_n| - |b|| &< | b_n - b| < \epsilon   \
        \end{align*}
        by reverse triangle inequality and \( (b_n) \to b\).
        \end{proof}
    \item[(c)] If \( (a_n) \to a\) and \( (b_n - a_n) \to 0\), then \( (b_n) \to a\).
        \begin{proof}
        Assume \( (a_n) \to a\) and \( (b_n - a_n) \to 0\). Let \( \epsilon  > 0\). By assumption, 
        \begin{align*}
            | a_n - a | &< \frac{ \epsilon }{2}  \text{,   \space  }  n \geq N_1\\
            | b_n - a_n | &< \frac{ \epsilon }{2} \text{, \space } n \geq N_2.
        \end{align*}
        Hence, choose \(  N = \max \{ N_1, N_2 \} \) such that 
        \begin{align*}
        | b_n - a |&= | b_n - a_n + a_n - a  | \\
                   &< | b_n - a_n | + | a_n - a | \\
                   &< \frac{ \epsilon }{2} + \frac{ \epsilon }{2} \\ 
                   &= \epsilon. 
        \end{align*}
        Hence, \( (b_n) \to a\).
        \end{proof}
    \item[(d)]If \( (a_n) \to a\) and \( | b_n - b | \leq a_n \) for all \( n \in \N \), then \( (b_n) \to b\).
        \begin{proof}
        Let \( \epsilon > 0\). Choose \( N \) so that \( a_n \to 0 \). Then consider \( |b_n - b |\) and observe that
        \begin{align*}
        | b_n - b| &\leq a_n < \epsilon, 
        \end{align*}
        Hence, it follows that \( (b_n ) \to b\).
        \end{proof}
\end{enumerate}

\subsubsection{Exercise 2.3.13(Iterated Limits).} Given a doubly indexed array \( a_{mn}\) where \( m, n \in \N \), what should \(\lim_{m,n \to \infty} a_{mn}\) represent?  

\begin{enumerate}
    \item[(a)] Let \( a_{mn} = m / (m+n)\)  and compute the \textit{iterated} Limits
        \[ \lim_{n \to \infty } \Big( \lim_{m \to \infty} a_{mn} \Big) \text{ and } \lim_{m \to \infty } \Big( \lim_{n \to \infty} a_{mn} \Big).\]
        Define \(\lim_{m,n \to \infty} a_{mn} = a \) to mean that for all \( \epsilon > 0 \) there exists an \( N \in \N \) such that if both \( m,n \geq N \), then \( |a_{mn} - a | < \epsilon \).
        \begin{proof}
        Let \( a_{mn} = m / (m+n)\). We can compute the \textit{iterated} limits 
        \[  \lim_{n \to \infty} \Big( \lim_{m \to \infty} \frac{m}{m+n}\Big) \tag{1}  \]
        and
        \[ \lim_{m \to \infty} \Big( \lim_{n \to \infty} \frac{m}{m+n}\Big). \tag{2}\]
        We start with (1). Hence, we have 
        \begin{align*}
            \lim_{n \to \infty } \Big( \lim_{ m \to \infty} \frac{m}{m+n}\Big)  &= \lim_{ n \to \infty} (1)  \\
                                                                                &= 1.
        \end{align*}
        With (2), we have 
        \begin{align*}
            \lim_{m \to \infty} \Big( \lim_{ n \to \infty} \frac{m}{m+n}\Big)&= \lim_{m \to \infty} (0) \\
                                                                             &= 0. 
        \end{align*}

        \end{proof}
    \item[(b)] Let \( a_{mn} = 1/(m+n)\). Does \( \lim_{m,n \to \infty} a_{mn} \) exist in this case? Do the two iterated limits exists? How do these three values compare? Answer these same questions for \( a_{mn} = mn / (m^2 + n^2 )\). 
        \begin{proof}
            Let us try and compute the limit of \( a_{mn} \) the same way we did above. Hence, we have 
            \[
                \lim_{n \to \infty} \Big( \lim_{m \to \infty} \frac{1}{m+n} \Big)= \lim_{n \to \infty} \Big( \lim_{ m \to \infty} \frac{1}{1 + n/m}\Big)= \lim_{ n \to \infty} (1) = 1 \tag{1}\\
            \]
            and 
            \[ \lim_{m \to \infty} \Big( \lim_{n \to \infty} \frac{1}{m+n} \Big) = 1. \tag{2}\]
            We claim that for \( \lim_{m,n \to  \infty} a_{mn}\) to exists, we have to have 
            \[ \lim_{n \to \infty} \Big( \lim_{m \to \infty} a_{mn}\Big) = \lim_{m \to \infty} \Big( \lim_{n \to \infty} a_{mn}\Big) \]
            hold. Since (1) and (2) are the equal to each other, we claim that \( \lim_{m,n \to  \infty} a_{mn}\) exists. 

            We can try to do the same process for the sequence \( a_{mn} = mn / (m^2 + n^2 )\). Hence, we have 
            \[ \lim_{n \to \infty} \Big( \lim_{m \to \infty} \frac{mn}{m^2 + n^2 } \Big) = \lim_{n \to \infty} (0) = 0 \tag{3} \]
            and 
            \[ \lim_{m \to \infty} \Big( \lim_{ n \to \infty} \frac{mn}{m^2 + n^2 } \Big) = \lim_{m \to \infty} (0)  = 0 \tag{4}\]
            Since (2) and (3) are equal, we have that \( \lim_{m,n \to  \infty} a_{mn}\) exists.  
        \end{proof}
    \item[(c)] Produce an example where \( \lim_{m,n \to \infty} a_{mn}\) exists but neither iterated limit can be computed. 
        \begin{proof}[Solution]
        Consider 
        \[ a_{m,n} = \frac{(-1)^n}{m} + \frac{(-1)^m}{n}\]
        where the iterated limits cannot be computed.
        \end{proof}
    \item Assume \( \lim_{m,n \to \infty} a_{mn} = a \), and assume that for each fixed \( m \in \N \), \( \lim_{n \to \infty} (a_{mn}) \to b_m \). Show \( \lim_{m \to \infty} b_m = a .\)
        \begin{proof}
            Suppose \( \lim_{m,n \to \infty} a_{mn} = a \), and assume that for each fixed \( m \in \N \), \( \lim_{n \to \infty } (a_{mn}) \to b_m \). We want to show that \( \lim_{m \to \infty } b_m = a \). Consider \( | b_m - a | \). Then fix \( m \in \N \) such that for any \( m,n \geq N \), we have that  
            \begin{align*}
                |b_m - a |&= |b_m - a_{mn} + a_{mn} - a | \\
                          &\leq |b_m - a_{mn}| + |a_{mn} - a | \\
                          &< \frac{\epsilon}{2} + \frac{\epsilon}{2} \\
                          &= \epsilon.
            \end{align*}
        Hence, \( (b_{m}) \to a \). 
        \end{proof}
\end{enumerate}
 







