\documentclass[a4paper]{report}
\usepackage{standalone}
\usepackage{import}

\input{../../../../../newpreamble.tex}


\begin{document}

\section{Lecture 3}

\subsection{Topics}

\begin{itemize}
    \item Polar Representation of complex numbers.
    \item Convergence of sequences in \( \C  \).
\end{itemize}

\subsection{Polar Representation of Complex Numbers}

First, let us introduce some notation:
\begin{itemize}
    \item \( \C^{\cdot} = \{ z \in \C : z \neq 0  \}. \)
    \item \( {\R}_{+} = \{ \alpha \in \R : \alpha > 0  \}. \)
\end{itemize}

Recall that any non-zero \( (\alpha , \beta ) \in \R^{2} \) can be represented as 
\[  (\alpha, \beta) = \gamma (\cos \varphi, \sin \varphi) \]
with \( \tan \varphi = \frac{ \beta  }{ \alpha }\).

Note that if \( \psi = 2 \pi + \varphi  \), then
\[  (\alpha , \beta ) = \gamma (\cos \psi , \sin \psi). \]

\begin{itemize}
    \item \( \gamma  \) is uniquely defined. 
    \item \( \varphi  \) is defined up to the addition of a multiple of \( 2 \pi  \).
\end{itemize}


\begin{remark}
    This representation may not be unique!
\end{remark}

\begin{prop}
   The map \( {\R}_{+} \times \R \to \C^{\cdot} \) defined by  
   \[  (\gamma, \varphi) \longrightarrow \gamma (\cos \varphi + i \sin \varphi ) \]
   is surjective.
\end{prop}

\begin{remark}
The proposition above is a systematic way of saying that if \( z \in \C^{\cdot} \), then     
\[  z = \gamma (\cos \varphi + i \sin \varphi ) \]
with \( \gamma = | z  |  \) and \( \varphi  \) can be determined up to a multiple of \( 2 \pi \).
\end{remark}

If we insist, we can make the polar representation unique by restricting the domain to \( -\pi < \varphi \leq \pi \) where \( \varphi  \) is denoted as the \textbf{argument of \( z  \)}.

\begin{definition}[Agument and Principle Argument]
    Let \( z \in \C^{\cdot} \) and \( z = \gamma (\cos \varphi + i \sin \varphi) \) be a polar representation of \( z  \). Then \( \varphi  \) is called \textbf{an argument of \( z  \)}. If \( - \pi < \varphi \leq \pi \), then \( \varphi  \) is called \textbf{the principal argument of \( z \)} and it is denoted by \( \Arg(z) \). 
\end{definition}
\begin{remark}
    For any other domain, we denote the argument by \( \varphi = \arg((x,y)) \).
\end{remark}

\begin{lemma}
    Let \( z = \gamma(\cos \varphi + i \sin \varphi) \) and \( w = \gamma' (\cos(\varphi') + \sin(\varphi') \) in \( \C \setminus  \{ 0  \}  \). Then
    \[  zw = \varphi \varphi' [\cos(\varphi + \varphi') + i \sin(\varphi + \varphi')]. \]
\end{lemma}
\begin{proof}
Using the addition formula, we can write
\begin{align*}
    zw &= \gamma \gamma'  (\cos \varphi + i \sin \varphi)(\cos \varphi' + i \sin \varphi')  \\
       &= \gamma \gamma' [ (\cos \varphi \cos \varphi' - \sin \varphi \sin \varphi') + i(\sin \varphi \cos \varphi' + \sin \varphi \cos \varphi') ] \\
       &= \gamma \gamma' (\cos(\varphi + \varphi') + i \sin(\varphi + \varphi')).
\end{align*}
\end{proof}

The proposition above allows us to visualize the multiplication of complex numbers as two parts:
    \begin{itemize}
        \item Scaling of the modulus.
        \item Addition of the two angles.
    \end{itemize}

\begin{corollary}
    Let \( z \in \C^{\cdot} \) with \( z = \gamma (\cos \varphi + i \sin \varphi) \). Then \begin{align*}
        z^{-1} &= \frac{ 1  }{  \gamma  }  ( \cos (- \varphi) + i \sin (- \varphi)) \\
               &= \frac{ 1 }{  \gamma  }  (\cos \varphi - i \sin \varphi).
    \end{align*}
\end{corollary}


\begin{corollary}[De Moivre's Theorem]
   Let \( z = \gamma (\cos \varphi + i \sin \varphi) \in \C \setminus  \{ 0 \}  \) and let \( n \in \Z   \). Then
   \[  z^{n} = \gamma^{n} (\cos n \varphi + i \sin n \varphi). \]
\end{corollary}

\begin{remark}
 If \( n  \) is a negative integer, then \( z^{n} = (z^{-1})^{-n} \). 
\end{remark}

The corollary above allows us to compute the \( n \)th roots of a non-zero complex number.

\begin{eg}[An example of De Moivre's Theorem]
   Suppose we had the complex number  
   \[  z = \frac{ 1 }{ 2 }  + i \frac{ \sqrt{ 3 }  }{ 2 }. \]
  Suppose we want to find \( z^{10} \). First, we need to find the angle that makes this complex number. Since the \( x  \) and \( y  \) coordinates are both positive this means that the angle must lie in the first quadrant. Thus, we have 
  \[  \varphi = \arg(z) = \frac{ \pi }{ 3  }. \]
  Using De Moivre's Theorem, we can write
  \begin{align*}
      z^{10 } &= \cos \Big(  10 \cdot \frac{ \pi  }{ 3 }  \Big) + i \sin \Big(  10 \cdot \frac{ \pi }{ 3 }  \Big) \\
              &= -\frac{1 }{ 2 }  - i \frac{ \sqrt{ 3 }  }{ 2 }. 
  \end{align*}
\end{eg}

Some notations we would like to establish are the following:
\begin{enumerate}
    \item[(i)] \textbf{The set of all positive real numbers} \( {\R}_{+} = \{ r \in \R : r > 0  \}  \)
    \item[(ii)] \textbf{The set of all complex numbers excluding zero} \( \C^{\cdot} =  \C \setminus \{ 0 \}  \).
\end{enumerate}

\begin{prop}
    The map \( {\R}_{+} \times \R \longrightarrow \C^{} \) defined by 
    \[  (r, \varphi) \longrightarrow \gamma ( \cos \varphi + i \sin \varphi) \]
    is surjective.
\end{prop}

\begin{remark}
    This gives us the tool we need to show that every non-zero \( z \in \C  \) has a polar representation.
\end{remark}

\subsection{Convergence of Sequences in \( \C \)}

\begin{definition}[Convergence in \( \C  \)]
    Let \( {\{ {z}_{n} \} }_{n=1}^{\infty }     \) be a sequence in \( \C  \). We say that \( \{ {z}_{n} \}   \) converges to \( z \in \C  \) if for all \(  \epsilon > 0  \), we can find \( {N}_{\epsilon} \in \N  \) such that  
    \[  | {z}_{n} - z  |  < \epsilon \]
    for all \( n \geq {N}_{\epsilon} \).
\end{definition}

If \( ({z}_{n}) \) converges to \( z  \), then we write \( {z}_{n} \to z  \).

\begin{prop}[Properties of Convergent Sequences]
   Assume \( ({z}_{n}) \to z  \) and \( ({w}_{n}) \to w   \). 
   \begin{enumerate}
       \item[(i)] Let \( \alpha, \beta \in \C  \), then \( \alpha {z}_{n} + \beta {w}_{n} \to \alpha z + \beta w  \).
        \item[(ii)] \( {z}_{n} {w}_{n} \to zw  \).
        \item[(iii)] \( {z}_{n}^{-1} \to z^{-1} \).
        \item[(iv)] \( ({z}_{n}) \to z  \) if and only if \( \Re({z}_{n}) \to \Re(z) \) and \( \Im({z}_{n}) \to \Im(z) \) as a sequences in \( \R  \).
   \end{enumerate}
\end{prop}
\begin{proof}
Suppose \( ({z}_{n}) \to z  \) and \( ({w}_{n}) \to w  \).
\begin{enumerate}
    \item[(i)] Let \( \alpha, \beta \in \C   \). Let \( \epsilon > 0  \). Since \( ({z}_{n}) \to z  \), there exists an \( {N}_{1} \in \N  \) such that for any \( n \geq {N}_{1} \), we have  
        \[  | {z}_{n} - z  |  < \frac{ \epsilon  }{ 2 \alpha }. \]
        Likewise, \( ({w}_{n}) \to w  \) implies that we can find an \( {N}_{2} \in \N  \) such that for any \( n \geq {N}_{2} \), we have
        \[  | {w}_{n} - w  |  < \frac{ \epsilon  }{ 2 \beta }. \]
        Now, choose \( N = \max \{ {N}_{1}, {N}_{2} \}  \). Then for any \( n \geq N  \), we must have 
        \begin{align*}
            | \alpha {z}_{n} + \beta {w}_{n} - (\alpha z + \beta w ) | &= |  \alpha ({z}_{n} - z ) + \beta ({w}_{n} - w )  |   \\
                                                                       &\leq \alpha | {z}_{n} - z | + \beta | {w}_{n} - w  | \\
                                                                       &< \alpha \cdot \frac{ \epsilon  }{ 2 \alpha }  + \beta \cdot \frac{ \epsilon  }{  2 \beta } \\
                                                                       &= \frac{ \epsilon  }{  2 }  + \frac{ \epsilon }{ 2 }  = \epsilon.
        \end{align*}
        Thus, we can conclude that 
        \[  \alpha {z}_{n} + \beta {w}_{n} \to \alpha z + \beta w.  \]
    \item[(ii)] Let \( \epsilon > 0  \). Our goal is to show that there exists an \( N \in \N  \) such that  
        \[  | {z}_{n} {w}_{n} - zw  |  < \epsilon. \]
        Since \( ({z}_{n}) \to z  \), we can find a \( {N}_{1} \in \N  \) such that for any \( n \geq {N}_{1} \), we have   
        \[  | {z}_{n} - z  |  < \frac{ \epsilon  }{  2 M   }   \]
        where \( M > 0  \).
        Since \( ({w}_{n})  \to w \), there exists \( {N}_{2} \in \N  \) such that for \( n \geq {N}_{2} \), we have 
        \[  | {w}_{n} - w  | < \frac{ \epsilon  }{  2 | z  |  }.  \]
        Thus, choose \( N = \max \{ {N}_{1}, {N}_{2} \}  \) such that for any \( n \geq N  \), we have
        \begin{align*}
            | {z}_{n} {w}_{n} - zw  |  &= | {z}_{n} {w}_{n} - {w}_{n} z + {w}_{n} z - zw  |  \\
                                       &\leq | {w}_{n}  | | {z}_{n} - z  | + | z  |  | {w}_{n} - w   | \\
                                       &\leq M | {z}_{n} - z  |  + | z  |  | {w}_{n} - w  |  \\
                                       &< M \cdot \frac{ \epsilon  }{ 2 M  }  + | z  |  \cdot \frac{ \epsilon  }{ 2 | z  |  }  \\
                                       &= \frac{ \epsilon  }{  2 }  + \frac{ \epsilon  }{  2  }  = \epsilon.
        \end{align*}
        Thus, we conclude that 
        \[ {z}_{n} {w}_{n} \to z w.  \]
    \item[(iii)] Let \( \epsilon > 0  \). We will show that \( {z}_{n}^{-1} \to z^{-1} \) by showing that there exists an \( N \in \N  \) such that for any \( n \geq N  \), we have 
        \[  | {z}_{n}^{-1} - z^{-1} | < \epsilon. \]
    Since \( ({z}_{n}) \to z  \), there must exists an \( {N}_{1} \in \N   \) such that for any \( n \geq {N}_{1}  \), we have
    \[  | {z}_{n} - z  |  < \frac{ \epsilon | z  |^{2} }{ 2 }.  \]
    Likewise, we can choose \( {N}_{2} \in \N  \) such that for any \( n \geq {N}_{2} \), we have
    \[  | {z}_{n}  |  > \frac{ | z |  }{ 2 }.  \]
    If we choose \( N = \max \{ {N}_{1}, {N}_{2} \}  \), and subsequently, let \( n \geq N  \), then we must have
    \begin{align*}
      | {z}_{n}^{-1} - z^{-1} |   &= \frac{ | {z}_{n} - z  |  }{  | z  |  | {z}_{n} |  } \\
                                  &< \frac{ \epsilon | z |^{2}  }{ 2  } \cdot \frac{ 2  }{  | z |^{2}  } \\ 
                                  &= \epsilon.
    \end{align*}
    Thus, we conclude that \( {z}_{n}^{-1} \to z^{-1} \).
\end{enumerate}
\end{proof}

\end{document}
