\documentclass[a4paper]{report}
\usepackage{standalone}
\usepackage{import}

\input{../../../../../newpreamble.tex}

\begin{document}

\section{Lecture 7}

\subsection{Topics}

Our goal for this lecture is to discuss complex powers of a non-zero complex number.

\subsection{Complex Powers}

Let \( z \in \C^{\bullet} \). We want to define \( z^{w} \) for \( w \in \C  \). Recall from real number system that, for \( x \in {\R}_{+} \), \( x^{a} = e^{a \ln x } \). We want our complex powers to extend this idea.

\begin{definition}[ ]
   We define \( z^{w} = \exp(w \log z) \). Note that  
   \begin{align*}
       \log z &= \Log z + 2 \pi i k  \\
              &= \ln | z  |  + i (\Arg(z) + 2\pi k), \ k \in \Z 
   \end{align*}
   is a multi-valued function.
\end{definition}

For this reason, the complex power of a non-zero complex number will also be multi-valued.
Hence, by choosing a fixed \( k  \), we can find a specific value of \( z^{w} \).

\begin{eg}
    \begin{enumerate}
        \item[(i)] Compute \( i^{i} \). Recall that \( \log i = i \Big(  \frac{ \pi  }{  2  }  + 2 \pi k  \Big) \). Hence, we have 
            \[  i^{i} = \exp(i \log i) = \{ e^{\frac{ -\pi }{ 2 }  + 2 \pi k }: k \in \Z  \}. \]
            If we are just referring to the principal branch, then 
            \[ i^{i} = e^{\frac{ -\pi }{ 2 } }.  \]
        \item[(ii)] Compute: \( (-1)^{1 + i} \).
            Note that 
            \[  \log(-1) = i \pi + 2 \pi i k  =  i (2k+1) \pi. \]
            Then we see that for all \( k \in \Z  \), we have
            \begin{align*}
                (-1)^{1 + i} &= \exp((2k+1)\pi (i-1)) \\
                             &= e^{-(2k+1)\pi} \exp(e^{(2k+1) \pi i }) \\
                             &= e^{-(2k+1)\pi} \Big[\cos (2k+1) \pi + i \sin (2k+1) \pi \Big] \\
                             &= - e^{-(2k+1)\pi}.
            \end{align*}
    \end{enumerate}
\end{eg}

Let us summarize some facts about \( \exp(z) \).

\begin{itemize}
    \item For all \( x \in \R  \), we have \( \exp(z) = e^{x} \). Thus, from now on, we write \( e^{z} \) in place of \( \exp(z) \).
    \item For \( z \in \C^{\bullet} \), we have \( \log z  \) is a multi-valued function. That is, we have 
        \[  \log z = \ln | z  |  + i (\Arg z + 2 \pi k ), \ k \in \Z.  \]
    \item For \( z \in \C^{\bullet} \), we have \( \Log z = \ln | z  |  + i \Arg z  \) (this is the principal branch log).
    \item For \( z \in \C^{\bullet} \), we have \( z^{w } = e^{w \log z} \) is also a multi-valued function.
\end{itemize}

\begin{eg}
    \begin{itemize}
        \item Find all solutions of \( \sin z = 1  \).
        \item Find all possible solutions of \( \cos z = i  \).
    \end{itemize}
\end{eg}

\begin{problem}
     Find all solutions of \( e^{z} = i  \).
\end{problem}
\begin{solution}

\end{solution}

\section{Lecture 8}

\begin{itemize}
    \item {\hyperref[Limits of a function]{Limits of a function}}  
    \item {\hyperref[Continuity]{Continuity}} 
    \item {\hyperref[Derivative]{Derivative}} 
\end{itemize}

\subsection{Functional Limit}\label{Limits of a function}

\begin{definition}[Functional Limit]
    Let \( D \subseteq \C   \) and \( f: D \to \C  \) be a function. Let \( a \) be an accumulation point of \( D  \). Let \( \ell \in \C  \). We say that \( \ell  \) is \textbf{the limit of \( f(z) \)} as \( z  \) approaches to \( a  \) if for all \( \epsilon > 0 \), there is \( \delta> 0  \) such that for all \( z \in D  \) with \( 0 < |  z - a  |  < \delta \), we have
    \[  | f(z) - \ell | < \epsilon; \]
    that is, \( z \in D \cap (B(a,\delta) \setminus  \{ a \} ) \) implies \( f(z) \in B(\ell, \epsilon) \).
\end{definition}

\begin{eg}
    Let \( f: B(0,1) \to \C  \) defined by \( f(z) = \frac{ iz }{ 2  }  \) then \( \lim_{ z \to i }  f(z) = - \frac{ 1 }{ 2 }  \).
\end{eg}
\begin{proof}
Observe that 
\[  | f(z) - \ell | = \Big| \frac{ i }{ 2 } z - \Big(  - \frac{ 1 }{ 2 }  \Big) \Big| = \Big| \frac{ i }{ 2 }  \Big|  | z - i  |  = \frac{ 1 }{ 2 }  | z - i  |.  \]
So, given any \( \epsilon > 0  \), we can take any \( 0 < \delta< 2 \epsilon  \) such that 
\[  0 < | z - i  | < \delta  \] implies 
\[  | f(z) - \ell | < \epsilon. \]
\end{proof}

Some facts about limits are:

\begin{theorem}[ ]
    Let \( D \subseteq \C  \) with \( f: D \to \C  \), \( g: D \to \C  \) be two functions let us write \( f = u + i v \).
    \begin{enumerate}
        \item[(i)] Let \( a = \alpha + i \beta \). Then \( \lim_{ z \to a  } f(x) = \ell \) if and only if 
        \begin{center}
            \( \lim_{ (x,y) \to (\alpha, \beta) } u(x,y) = \Re(\ell)  \) and \( \lim_{ (x,y) \to (\alpha, \beta)  } v(x,y) = \Im(\ell) \); that is,
            \[  \lim_{ z \to a }  f(z) = \lim_{ z \to a }  u(z) + i \lim_{ z \to a } v(z). \] 
        \end{center}
    \item[(ii)] Let \( \lim_{ z \to  a  }  f(z) = \ell  \) and \( \lim_{ z \to a } g(z) = \ell' \) and \( c,d \in \C  \). Then
        \[  \lim_{ z \to a }  (cf(z) + dg(z)) = c \ell + d \ell'.  \]
    \item[(iii)] \( \lim_{ z \to a } (f(z)g(z)) = \lim_{ z \to a } f(z) \cdot \lim_{ z \to a }  g(z) \).
    \item[(iv)] We have
        \[  \lim_{ z \to a }  \frac{ f(z) }{ g(z) }  = \frac{ \lim_{ z \to a }  f(z) }{ \lim_{ z \to a } g(z) }  \]
        whenever \( \lim_{ z \to a } g(z) \neq 0  \).
    \end{enumerate}
\end{theorem}

\begin{problem}
    Let \( \lim_{ z \to i } f(z) = 2 + i    \) and \( \lim_{ z \to i }  g(z) = 1 - i  \). Compute the following:
    \[ \lim_{ z \to i }  \Big[ (f(z))^{3} + \frac{ (1+i) g(z) }{ z^{2} } \Big]. \]
\end{problem} 
\begin{solution}
Observe that 
\begin{align*}
  \lim_{ z \to i }  \Big[(f(z))^{3} + \frac{ (1+i) g(z) }{ z^{2} } \Big]  &= \lim_{ z \to i }  (f(z))^{3} + \lim_{ z \to i }  \frac{ (1+i) g(z)  }{ z^{2} }  \\
                                                                          &= (2+i)^{3} + \frac{ (1+i) (1-i) }{ i^{2} } \\
                                                                          &= (2+i)^{3} -2. 
\end{align*}
\end{solution}

\begin{definition}[Limits at Infinity]
    \begin{enumerate}
        \item[(i)] Let \( f: D \to \C  \) be a function and \( a \in \C  \) be an accumulation point of \( D  \). Then we say \( \lim_{ z \to a } f(z) = \infty   \) if for all \( M > 0  \), there exists \( \delta > 0  \) such that
            \[  z \in D \cap (B(a,\delta) \setminus  \{ a \} ) \]
            implies \( | f(z) | \geq  M \); that is, \( f  \) is unbounded as \( z  \) approaches to \( a  \).
        \item[(ii)] Let \( f  \) be a complex function defined on the complement of a ball in \( \C  \). We say \( \lim_{ z \to \infty  } f(z) = \ell  \) if for all \( \epsilon > 0  \), there exists \( R > 0  \) such that \( | z  |  > R  \) implies 
            \[  | f(z) - \ell  | < \epsilon. \]
    \end{enumerate}
\end{definition}

\begin{eg}
    \begin{enumerate}
        \item[(i)] Consider \( \lim_{ z \to 0 }  \frac{ 1 }{ z }  = \infty   \). Let \( M > 0  \). Let \( \delta = \frac{ 1 }{ M }  \). Then \( 0 < | z  |  < \delta \) implies that 
            \[  \Big| \frac{ 1 }{ z }  \Big| > \frac{ 1 }{ \delta } = M. \]
        \item[(ii)] Consider \( \lim_{ z \to \infty  }   \frac{ 1 }{ z }  = 0.  \)
            Let \( \epsilon > 0  \). Choose \( R = \frac{ 1 }{ \epsilon } > 0  \). Then 
            \(  | z  |  > R  \) implies 
            \[  \Big| \frac{ 1 }{ z }  \Big| < \frac{ 1 }{ R } = \epsilon. \]
    \end{enumerate}
\end{eg}

\begin{problem}
    \begin{enumerate}
        \item[(i)] Show that \( \lim_{ z \to \infty  } f(z) = \ell  \) if and only if
            \[  \lim_{ z \to \infty  } f \Big(  \frac{ 1 }{ z }  \Big) = \ell.  \]
        \item[(ii)] \( \lim_{ z \to a } f(z) = \infty   \) if and only if \( \lim_{ z \to a }  \frac{ 1 }{ f(z) } = 0  \).
        \item[(iii)] Give a definition of \( \lim_{ z \to \infty  } f(z) = \infty   \). Show that \( \lim_{ z \to \infty  } f(z) = \infty  \) if and only if \( \lim_{ z \to 0 } f \Big(  \frac{ 1 }{ z }  \Big) = \infty  \).
        \item[(iv)] Compute \( \lim_{ z \to \infty  }  \frac{ z - 1  }{ z + i  }  \).
        \item[(v)] Compute \( \lim_{ z \to \infty    }  \frac{ gz + i  }{ z^{2} + z + 1  }  \). 
        \item[(vi)] Can you compute \( \lim_{ z \to \infty   }  e^{-z}  \)?
    \end{enumerate}
\end{problem}

\subsection{Continuity}\label{Continuity}

\begin{definition}[Continuity]
    Let \( D \subseteq \C   \) and \( f: D \to \C  \) be a function. We say \textbf{\( f  \) is continuous at \( a \in D  \)} if for all \( \epsilon > 0  \), there exists \( \delta > 0  \) such that for all \( z \in B(a,\delta) \cap D \), we have \( f(z) \in B(f(a), \epsilon) \).
\end{definition}

\begin{eg}
    Compute \( \lim_{ z \to \infty   }  \frac{ z - i  }{  z + i  }  \). Observe that 
    \begin{align*}
        \lim_{ w \to 0 } \frac{ \frac{ 1 }{ w }  - i  }{  \frac{ 1 }{ w }  + i  } &= \lim_{ w \to 0 }  \frac{ 1 - wi }{  1+ wi }  
                                                                                  = 1.
    \end{align*}
\end{eg}

\begin{lemma}
    Let \( f: D \to \C  \) be a function. Then the following statements are equivalent.
    \begin{enumerate}
        \item[(i)] If \( f  \) is continuous at \( a \in D  \).
        \item[(ii)] For any sequence \( ({a}_{n}) \) and \( {a}_{n} \in D  \) such that \( {a}_{n} \to a  \), we have
            \[  f({a}_{n})  \to f(a).\]
    \end{enumerate}
    We say that \( f: D \to \C  \) is continuous if \( f  \) is continuous if \( f  \) is continuous for every \( a \in D  \).
\end{lemma}

Some facts that we can prove as an exercise:

\begin{lemma}
Let \( f: D \to \C  \) with \( D \subseteq \C \). Then we have
\begin{enumerate}
    \item[(1)] \( f  \) is continuous if and only if \( \Re(f) \) and \( \Im(f) \) are continuous (Note that \( \Re(f) \) and \( \Im(f) \) are functions of two variables in \( \R  \); that is, \( \Re(f) : D \to \R  \) an \( \Im(f) : D \to \R  \) ).
    \item[(2)] Linear combinations and products of continuous functions are continuous.
    \item[(3)] Composition of functions are continuous. 
    \item[(4)] If \( f  \) is continuous on \( D  \) and \( f(z) \neq 0  \) for all \( z \in D  \), then \( \frac{ 1 }{ f }  \) is continuous on \( D  \).
    \item[(5)] If \( f  \) is continuous, then \( | f |   \) is also continuous (note that \( | f |  = \sqrt{ (\Re(f))^{2} + (\Im(f))^{2} }  \)).
\end{enumerate}
\end{lemma}
\begin{proof}
\textbf{Left as an exercise.}
\end{proof}

\begin{eg}
    \begin{enumerate}
        \item[(1)] \( \exp: \C \to \C^{\bullet} \) is continuous.
        \item[(2)] \( \sin, \cos, \sinh, \cosh \) are all continuous.
        \item[(3)] \( \Arg: \C^{\bullet} \to (-\pi, \pi] \) is continuous on \( \C_{-} = \C^{\bullet} \setminus  \{ \text{negative real axis} \}  \) (\textbf{this will be on the next homework}).
        \item[(4)] \( \Log: \C^{\bullet} \to \{ x + iy: -\pi < y \leq \pi  \}  \) is continuous on \( \C_{-} \) (\textbf{this will be on the next homework})
        \item[(5)] \( \Arg  \) and \( \Log  \) are both not continuous at any \( z < 0  \) (that is, points on negative axis).
        \item[(6)] Fix \( {a}_{0}, {a}_{1}, \dots, {a}_{n} \in \C  \). Then
            \[  f(z) = {a}_{0} + {a}_{1} z + \cdots + {a}_{n} {z}_{n} \]
            is continuous on \( \C  \); that is, any polynomial with complex coefficients will be continuous.
    \end{enumerate}
\end{eg}

Note that \( \Arg: \C^{\bullet} \to (-\pi, \pi] \subseteq  \R \subseteq \C  \) is a discontinuous.

\subsection{Complex Derivative}\label{Derivative}

\begin{lemma}
    Let \( f: D \to \C  \) be a function and \( a \) is an accumulation point of \( D  \). Then the following statements are equivalent.
    \begin{enumerate}
        \item[(1)] \( \lim_{ z \to a } f(z) = \ell  \)
        \item[(2)] Define \( \tilde{f} : D \cup \{ a \} \to \C   \) by
                \[  \tilde{f}(z) = 
                \begin{cases}
                    f(z) &\text{if} \ z \in D \\
                    \ell &\text{if} \ z = a.
                \end{cases} \]
            Then \( \tilde{f} \) is continuous at \( a  \).
    \end{enumerate}
\end{lemma}
The reason we define (2) the way it is is because we may have a removable discontinuity.


We will us the lemma above to define complex differentiability.

\begin{definition}[Differentiability]
    Let \( f: D \to \C  \) be a function and \( a \in D  \) such that \( a \) is an accumulation point of \( D \setminus  \{ a \}  \). We say that \( f  \) is differentiable at \( a  \) if  
    \[  \lim_{ z \to a }  \frac{ f(z) - f(a) }{ z -a  } \ \text{exists}.  \] 
    If \( f  \) is differentiable at \( a \), we denote this limit by \( f'(a) \). We say \( f  \) is differentiable on \( D  \) if \( f  \) is differentiable at each \( a \in D  \). In this case, we can define a new function \( f': D \to \C  \) where \( z \mapsto f'(z) \).
\end{definition}







\end{document}
